Change hocap rand to not need invariants

theories/coneris/examples/random_counter/impl1.v
@@ -1,6 +1,6 @@
 From iris.algebra Require Import frac_auth.
 From iris.base_logic.lib Require Import invariants.
-From clutch.coneris Require Import coneris hocap hocap_rand random_counter.
+From clutch.coneris Require Import coneris hocap_rand random_counter.
 
 Set Default Proof Using "Type*".
 
@@ -15,31 +15,30 @@ Section impl1.
                                    counterG1_frac_authR:: inG Σ (frac_authR natR) }.
 
   Definition counter_inv_pred1 c γ2 := (∃ (l:loc) (z:nat), ⌜c=#l⌝ ∗ l ↦ #z ∗ own γ2 (●F z) )%I.
-  Definition is_counter1 N (c:val) γ1 γ2:=
-    (is_rand (L:=L) (N.@"rand") γ1 ∗
-    inv (N.@"counter") (counter_inv_pred1 c γ2)
+  Definition is_counter1 N (c:val) γ1:=
+    (
+    inv (N) (counter_inv_pred1 c γ1)
     )%I.
 
   Lemma new_counter_spec1 E N:
     {{{ True }}}
       new_counter1 #() @ E
       {{{ (c:val), RET c;
-          ∃ γ1 γ2, is_counter1 N c γ1 γ2 ∗ own γ2 (◯F 0%nat)
+          ∃ γ1, is_counter1 N c γ1 ∗ own γ1 (◯F 0%nat)
       }}}.
   Proof.
     rewrite /new_counter1.
     iIntros (Φ) "_ HΦ".
     wp_pures.
-    iMod (rand_inv_create_spec) as "(%γ1 & #Hinv)".
+    (* iMod (rand_inv_create_spec) as "(%γ1 & #Hinv)". *)
     wp_alloc l as "Hl".
-    iMod (own_alloc (●F 0%nat ⋅ ◯F 0%nat)) as "[%γ2[H5 H6]]".
+    iMod (own_alloc (●F 0%nat ⋅ ◯F 0%nat)) as "[%γ1[H5 H6]]".
     { by apply frac_auth_valid. }
     replace (#0) with (#0%nat) by done.
-    iMod (inv_alloc _ _ (counter_inv_pred1 (#l) γ2) with "[$Hl $H5]") as "#Hinv'"; first done.
+    iMod (inv_alloc _ _ (counter_inv_pred1 (#l) γ1) with "[$Hl $H5]") as "#Hinv'"; first done.
     iApply "HΦ".
     iFrame.
-    iModIntro.
-    iExists _. by iSplit.
+    by iModIntro.
   Qed.
 
   (* (** Not used in instantiating type class*) *)
@@ -83,89 +82,89 @@ Section impl1.
   (*   by iApply "HΦ". *)
   (* Qed. *)
 
-  Lemma allocate_tape_spec1 N E c γ1 γ2:
+  Lemma allocate_tape_spec1 N E c γ1:
     ↑N ⊆ E->
-    {{{ is_counter1 N c γ1 γ2 }}}
+    {{{ is_counter1 N c γ1 }}}
       allocate_tape1 #() @ E
-      {{{ (v:val), RET v;
-          ∃ (α:loc), ⌜v=#lbl:α⌝ ∗ rand_tapes_frag (L:=L) γ1 α (3%nat, [])
+      {{{ (v:val), RET v; rand_tapes (L:=L) v (3%nat, [])
       }}}.
   Proof.
-    iIntros (Hsubset Φ) "[#Hinv #Hinv'] HΦ".
+    iIntros (Hsubset Φ) "#Hinv HΦ".
     rewrite /allocate_tape1.
     wp_pures.
-    wp_apply rand_allocate_tape_spec; [by eapply nclose_subseteq'|done..].
+    by wp_apply rand_allocate_tape_spec. 
   Qed.
 
-  Lemma incr_counter_tape_spec_some1 N E c γ1 γ2 (Q:nat->iProp Σ) (α:loc) n ns:
+  Lemma incr_counter_tape_spec_some1 N E c γ1 (Q:nat->iProp Σ) α n ns:
     ↑N⊆E ->
-    {{{ is_counter1 N c γ1 γ2 ∗
-        rand_tapes_frag (L:=L) γ1 α (3, n::ns) ∗
-        (  ∀ (z:nat), own γ2 (●F z) ={E∖↑N}=∗
-                    own γ2 (●F (z+n)) ∗ Q z)
+    {{{ is_counter1 N c γ1 ∗
+        rand_tapes (L:=L) α (3, n::ns) ∗
+        (  ∀ (z:nat), own γ1 (●F z) ={E∖↑N}=∗
+                    own γ1 (●F (z+n)) ∗ Q z)
            
     }}}
-      incr_counter_tape1 c #lbl:α @ E
-                                 {{{ (z:nat), RET (#z, #n); rand_tapes_frag (L:=L) γ1 α (3, ns) ∗
+      incr_counter_tape1 c α @ E
+                                 {{{ (z:nat), RET (#z, #n); rand_tapes (L:=L) α (3, ns) ∗
                                                           Q z }}}.
   Proof.
-    iIntros (Hsubset Φ) "([#Hinv #Hinv'] & Hfrag & Hvs) HΦ".
+    iIntros (Hsubset Φ) "(#Hinv & Hfrag & Hvs) HΦ".
     rewrite /incr_counter_tape1.
     wp_pures.
-    wp_apply (rand_tape_spec_some with "[$]") as "Hfrag"; first by eapply nclose_subseteq'. 
+    wp_apply (rand_tape_spec_some with "[$]") as "Hfrag". 
     wp_pures.
     wp_bind (FAA _ _).
-    iInv "Hinv'" as ">(%&%&-> & ?&?)" "Hclose".
+    iInv "Hinv" as ">(%&%&-> & ?&?)" "Hclose".
     wp_faa.
-    iMod (fupd_mask_subseteq (E ∖ ↑N)) as "Hclose'".
-    + apply difference_mono_l.
-      by apply nclose_subseteq'.
-    + iMod ("Hvs" with "[$]") as "[? HQ]".
-      iMod "Hclose'" as "_".
-      rewrite -Nat2Z.inj_add.
-      iMod ("Hclose" with "[-HQ Hfrag HΦ]") as "_"; first by iFrame.
-      iModIntro.
-      wp_pures.
-      iApply "HΦ". by iFrame.
+    (* iMod (fupd_mask_subseteq (E ∖ ↑N)) as "Hclose'". *)
+    (* + apply difference_mono_l. *)
+    (*   by apply nclose_subseteq'. *)
+    (* +  *)
+    iMod ("Hvs" with "[$]") as "[? HQ]".
+    (* iMod "Hclose'" as "_". *)
+    rewrite -Nat2Z.inj_add.
+    iMod ("Hclose" with "[-HQ Hfrag HΦ]") as "_"; first by iFrame.
+    iModIntro.
+    wp_pures.
+    iApply "HΦ". by iFrame.
   Qed.
 
-  Lemma counter_tapes_presample1 N E γ1 γ2 c α ns ε (ε2 : fin 4%nat -> R):
+  Lemma counter_tapes_presample1 N E γ1 c α ns ε (ε2 : fin 4%nat -> R):
     ↑N ⊆ E ->
     (∀ x, 0<=ε2 x)%R ->
     (SeriesC (λ n, 1 / 4 * ε2 n)%R <= ε)%R ->
-    is_counter1 N c γ1 γ2  -∗
-    rand_tapes_frag (L:=L) γ1 α (3%nat, ns) -∗
+    is_counter1 N c γ1 -∗
+    rand_tapes (L:=L) α (3%nat, ns) -∗
     ↯ ε  -∗
-    state_update E (∃ n, ↯ (ε2 n) ∗ rand_tapes_frag (L:=L) γ1 α (3%nat, ns++[fin_to_nat n])).
+    state_update E (∃ n, ↯ (ε2 n) ∗ rand_tapes (L:=L) α (3%nat, ns++[fin_to_nat n])).
   Proof.
-    iIntros (Hsubset Hpos Hineq) "[#Hinv #Hinv'] Hfrag Herr".
-    iMod (rand_tapes_presample with "[//][$][$]") as "(%&$&$)"; try done; first by apply nclose_subseteq'.
+    iIntros (Hsubset Hpos Hineq) "#Hinv Hfrag Herr".
+    iMod (rand_tapes_presample with "[$][$]") as "(%&$&$)"; try done.
     etrans; last exact.
     apply Req_le.
     apply SeriesC_ext; intros. simpl. lra.
   Qed.
   
-  Lemma read_counter_spec1 N E c γ1 γ2 Q:
+  Lemma read_counter_spec1 N E c γ1 Q:
     ↑N ⊆ E ->
-    {{{  is_counter1 N c γ1 γ2  ∗
-         (∀ (z:nat), own γ2 (●F z) ={E∖↑N}=∗
-                     own γ2 (●F z) ∗ Q z)
+    {{{  is_counter1 N c γ1 ∗
+         (∀ (z:nat), own γ1 (●F z) ={E∖↑N}=∗
+                     own γ1 (●F z) ∗ Q z)
         
     }}}
       read_counter1 c @ E
       {{{ (n':nat), RET #n'; Q n'
       }}}.
   Proof.
-    iIntros (Hsubset Φ) "([#Hinv #Hinv'] & Hvs) HΦ".
+    iIntros (Hsubset Φ) "(#Hinv & Hvs) HΦ".
     rewrite /read_counter1.
     wp_pure.
-    iInv "Hinv'" as ">( %l & %z & -> & H5 & H6)" "Hclose".
+    iInv "Hinv" as ">( %l & %z & -> & H5 & H6)" "Hclose".
     wp_load.
-    iMod (fupd_mask_subseteq (E ∖ ↑N)) as "Hclose'".
-    { apply difference_mono_l.
-      by apply nclose_subseteq'. }
+    (* iMod (fupd_mask_subseteq (E ∖ ↑N)) as "Hclose'". *)
+    (* { apply difference_mono_l. *)
+    (*   by apply nclose_subseteq'. } *)
     iMod ("Hvs" with "[$]") as "[? HQ]".
-    iMod "Hclose'" as "_".
+    (* iMod "Hclose'" as "_". *)
     iMod ("Hclose" with "[-HQ HΦ]"); first by iFrame.
     iApply ("HΦ" with "[$]").
   Qed.
@@ -178,47 +177,47 @@ Program Definition random_counter1 `{!conerisGS Σ, F:rand_spec}: random_counter
     incr_counter_tape := incr_counter_tape1;
     read_counter:=read_counter1;
     counterG := counterG1;
-    tape_name := rand_tape_name;
+    (* tape_name := rand_tape_name; *)
     counter_name :=gname;
-    is_counter _ N c γ1 γ2 := is_counter1 (L:=counterG1_randG) N c γ1 γ2;
-    counter_tapes_auth _ γ m :=  rand_tapes_auth (L:=counterG1_randG) γ ((λ ns, (3, ns))<$>m);
-    counter_tapes_frag _ γ α ns := rand_tapes_frag (L:= counterG1_randG)γ α (3%nat, ns);
+    is_counter _ N c γ1 := is_counter1 N c γ1;
+    (* counter_tapes_auth _ γ m :=  rand_tapes_auth (L:=counterG1_randG) γ ((λ ns, (3, ns))<$>m); *)
+    counter_tapes _  α ns := rand_tapes (L:= counterG1_randG) α (3%nat, ns);
     counter_content_auth _ γ z := own γ (●F z);
     counter_content_frag _ γ f z := own γ (◯F{f} z);
     counter_tapes_presample _ := counter_tapes_presample1;
-    new_counter_spec _ := new_counter_spec1;
+    new_counter_spec _ := new_counter_spec1 (L:=counterG1_randG);
     allocate_tape_spec _ :=allocate_tape_spec1;
     incr_counter_tape_spec_some _ :=incr_counter_tape_spec_some1;
-    read_counter_spec _ :=read_counter_spec1
+    read_counter_spec _ :=read_counter_spec1 (L:=counterG1_randG)
   |}.
-Next Obligation.
-  simpl.
-  iIntros (?????????) "H1 H2".
-  iDestruct (rand_tapes_auth_exclusive with "[$][$]") as "[]".
-Qed.
-Next Obligation.
-  simpl.
-  iIntros.
-  iDestruct (rand_tapes_frag_exclusive with "[$][$]") as "[]".
-Qed.
+(* Next Obligation. *)
+(*   simpl. *)
+(*   iIntros (?????????) "H1 H2". *)
+(*   iDestruct (rand_tapes_auth_exclusive with "[$][$]") as "[]". *)
+(* Qed. *)
 Next Obligation.
   simpl.
   iIntros.
-  iDestruct (rand_tapes_agree with "[$][$]") as "%H".
-  iPureIntro.
-  apply lookup_fmap_Some in H as (?&?&?).
-  by simplify_eq.
+  iDestruct (rand_tapes_exclusive with "[$][$]") as "[]".
 Qed.
+(* Next Obligation. *)
+(*   simpl. *)
+(*   iIntros. *)
+(*   iDestruct (rand_tapes_agree with "[$][$]") as "%H". *)
+(*   iPureIntro. *)
+(*   apply lookup_fmap_Some in H as (?&?&?). *)
+(*   by simplify_eq. *)
+(* Qed. *)
 Next Obligation.
   iIntros.
   iDestruct (rand_tapes_valid with "[$]") as "$".
 Qed.
-Next Obligation.
-  simpl.
-  iIntros.
-  iMod (rand_tapes_update with "[$][$]") as "[??]"; last iFrame; first done.
-  by rewrite fmap_insert.
-Qed.
+(* Next Obligation. *)
+(*   simpl. *)
+(*   iIntros. *)
+(*   iMod (rand_tapes_update with "[$][$]") as "[??]"; last iFrame; first done. *)
+(*   by rewrite fmap_insert. *)
+(* Qed. *)
 Next Obligation.
   simpl.
   iIntros (?????????) "H1 H2".
